Iris/Iris/Algebra/Lib/DFracAgree.lean
@@ -55,23 +55,19 @@ theorem mk_injN {d₁ d₂ : DFrac} {a₁ a₂ : A} (h : mk d₁ a₁ ≡{n}≡ 
   ⟨h.1, toAgree.inj h.2⟩
 
 @[rocq_alias to_dfrac_agree_inj]
-theorem mk_inj {d₁ d₂ : DFrac} {a₁ a₂ : A} (h : mk d₁ a₁ ≡ mk d₂ a₂) : d₁ ≡ d₂ ∧ a₁ ≡ a₂ :=
-  ⟨fun n => (h n).1, Agree.toAgree_inj fun n => (h n).2⟩
+theorem mk_inj {d₁ d₂ : DFrac} {a₁ a₂ : A} (h : mk d₁ a₁ ≡ mk d₂ a₂) : d₁ = d₂ ∧ a₁ = a₂ :=
+  ⟨OFE.Equiv.to_eq fun n => (h n).1, Agree.toAgree_inj fun n => (h n).2⟩
 
 @[rocq_alias dfrac_agree_op]
-theorem mk_op {d₁ d₂ : DFrac} {a : A} : mk (d₁ • d₂) a ≡ mk d₁ a • mk d₂ a :=
-  NonExpansive₂.eqv Equiv.rfl Agree.idemp.symm
+theorem mk_op {d₁ d₂ : DFrac} {a : A} : mk (d₁ • d₂) a = mk d₁ a • mk d₂ a :=
+  equiv_prod_ext rfl Agree.idemp.symm
 
 @[rocq_alias dfrac_agree_op_valid]
-theorem op_valid {d₁ d₂ : DFrac} {a₁ a₂ : A} : ✓ (mk d₁ a₁ • mk d₂ a₂) ↔ ✓ (d₁ • d₂) ∧ a₁ ≡ a₂ := by
+theorem op_valid {d₁ d₂ : DFrac} {a₁ a₂ : A} : ✓ (mk d₁ a₁ • mk d₂ a₂) ↔ ✓ (d₁ • d₂) ∧ a₁ = a₂ := by
   simp only [Valid, Prod.Valid, Prod.op, CMRA.op, mk]
-  exact and_congr_right fun _ => Agree.toAgree_op_valid_iff_equiv
+  exact and_congr_right fun _ => toAgree_op_valid_iff_eq
 
-@[rocq_alias dfrac_agree_op_valid_L]
-theorem op_valid_L {d₁ d₂ : DFrac} {a₁ a₂ : A} :
-    ✓ (mk d₁ a₁ • mk d₂ a₂) ↔ ✓ (d₁ • d₂) ∧ a₁ = a₂ := by
-  rw [op_valid]
-  exact and_congr_right fun _ => ⟨OFE.Equiv.to_eq, OFE.Equiv.of_eq⟩
+#rocq_ignore dfrac_agree_op_valid_L "Use op_valid"
 
 @[rocq_alias dfrac_agree_op_validN]
 theorem op_validN {d₁ d₂ : DFrac} {a₁ a₂ : A} :
@@ -83,21 +79,17 @@ theorem op_validN {d₁ d₂ : DFrac} {a₁ a₂ : A} :
 
 @[rocq_alias dfrac_agree_included]
 theorem included {d₁ d₂ : DFrac} {a₁ a₂ : A} :
-    mk d₁ a₁ ≼ mk d₂ a₂ ↔ (d₁ ≼ d₂) ∧ a₁ ≡ a₂ := by
+    mk d₁ a₁ ≼ mk d₂ a₂ ↔ (d₁ ≼ d₂) ∧ a₁ = a₂ := by
   simp only [mk, Included]
   constructor
   · rintro ⟨⟨zd, za⟩, H⟩
-    exact ⟨⟨zd, fun n => (H n).1⟩, Agree.toAgree_included.mp ⟨za, fun n => (H n).2⟩⟩
+    exact ⟨⟨zd, congrArg Prod.fst H⟩,
+      Agree.toAgree_included.mp ⟨za, congrArg Prod.snd H⟩⟩
   · rintro ⟨⟨zd, hd⟩, ha⟩
-    refine ⟨(zd, toAgree a₁), NonExpansive₂.eqv hd ?_⟩
-    show toAgree a₂ ≡ toAgree a₁ • toAgree a₁
-    exact (NonExpansive.eqv ha.symm).trans Agree.idemp.symm
+    refine ⟨(zd, toAgree a₁), equiv_prod_ext hd ?_⟩
+    exact (congrArg toAgree ha.symm).trans Agree.idemp.symm
 
-@[rocq_alias dfrac_agree_included_L]
-theorem included_L {d₁ d₂ : DFrac} {a₁ a₂ : A} :
-    mk d₁ a₁ ≼ mk d₂ a₂ ↔ (d₁ ≼ d₂) ∧ a₁ = a₂ := by
-  rw [included]
-  exact and_congr_right fun _ => ⟨OFE.Equiv.to_eq, OFE.Equiv.of_eq⟩
+#rocq_ignore dfrac_agree_included_L "Use included"
 
 @[rocq_alias dfrac_agree_includedN]
 theorem includedN {d₁ d₂ : DFrac} {a₁ a₂ : A} :
@@ -108,7 +100,7 @@ theorem includedN {d₁ d₂ : DFrac} {a₁ a₂ : A} :
     exact ⟨(inc_iff_incN (α := DFrac) n).mpr ⟨zd, hd⟩, Agree.toAgree_includedN.mp ⟨za, ha⟩⟩
   · rintro ⟨hdinc, ha⟩
     obtain ⟨zd, hd⟩ := (inc_iff_incN (α := DFrac) n).mp hdinc
-    exact ⟨(zd, toAgree a₁), hd, (toAgree.ne.ne ha.symm).trans (Equiv.dist Agree.idemp.symm)⟩
+    exact ⟨(zd, toAgree a₁), hd, (toAgree.ne.ne ha.symm).trans Agree.idemp.symm.dist⟩
 
 @[rocq_alias dfrac_agree_update_2]
 theorem update₂ {d₁ d₂ : DFrac} {a₁ a₂ a' : A} (hd : d₁ • d₂ = .own 1) :
@@ -119,7 +111,7 @@ theorem update₂ {d₁ d₂ : DFrac} {a₁ a₂ a' : A} (hd : d₁ • d₂ = .
     _ ≡ (own (1 : Qp), toAgree a₁ • toAgree a₂) := this
     _ ~~> mk d₁ a' • mk d₂ a' :=
       @Update.exclusive _ _ _ _ one_exclusive_left
-        (op_valid.mpr ⟨hd ▸ valid_own_one, .rfl⟩)
+        (op_valid.mpr ⟨hd ▸ valid_own_one, rfl⟩)
 
 @[rocq_alias dfrac_agree_persist]
 theorem persist {d : DFrac} {a : A} : mk d a ~~> mk .discard a := by
@@ -150,16 +142,14 @@ def mk [OFE A] (q : Qp) (a : A) : DFracAgreeR A := DFracAgree.mk (.own q) a
 variable {A : Type _} [OFE A]
 
 @[rocq_alias frac_agree_op]
-theorem mk_op {q₁ q₂ : Qp} {a : A} : mk (q₁ + q₂) a ≡ mk q₁ a • mk q₂ a :=
+theorem mk_op {q₁ q₂ : Qp} {a : A} : mk (q₁ + q₂) a = mk q₁ a • mk q₂ a :=
   DFracAgree.mk_op (d₁ := .own q₁) (d₂ := .own q₂)
 
 @[rocq_alias frac_agree_op_valid]
 theorem op_valid {q₁ q₂ : Qp} {a₁ a₂ : A} :
-    ✓ (mk q₁ a₁ • mk q₂ a₂) ↔ (q₁ + q₂).val ≤ 1 ∧ a₁ ≡ a₂ := DFracAgree.op_valid
+    ✓ (mk q₁ a₁ • mk q₂ a₂) ↔ (q₁ + q₂).val ≤ 1 ∧ a₁ = a₂ := DFracAgree.op_valid
 
-@[rocq_alias frac_agree_op_valid_L]
-theorem op_valid_L {q₁ q₂ : Qp} {a₁ a₂ : A} :
-    ✓ (mk q₁ a₁ • mk q₂ a₂) ↔ (q₁ + q₂).val ≤ 1 ∧ a₁ = a₂ := DFracAgree.op_valid_L
+#rocq_ignore frac_agree_op_valid_L "Use op_valid"
 
 @[rocq_alias frac_agree_op_validN]
 theorem op_validN {q₁ q₂ : Qp} {a₁ a₂ : A} :
@@ -168,11 +158,9 @@ theorem op_validN {q₁ q₂ : Qp} {a₁ a₂ : A} :
 
 @[rocq_alias frac_agree_included]
 theorem included {q₁ q₂ : Qp} {a₁ a₂ : A} :
-    mk q₁ a₁ ≼ mk q₂ a₂ ↔ (own q₁ ≼ own q₂) ∧ a₁ ≡ a₂ := DFracAgree.included
+    mk q₁ a₁ ≼ mk q₂ a₂ ↔ (own q₁ ≼ own q₂) ∧ a₁ = a₂ := DFracAgree.included
 
-@[rocq_alias frac_agree_included_L]
-theorem included_L {q₁ q₂ : Qp} {a₁ a₂ : A} :
-    mk q₁ a₁ ≼ mk q₂ a₂ ↔ (own q₁ ≼ own q₂) ∧ a₁ = a₂ := DFracAgree.included_L
+#rocq_ignore frac_agree_included_L "Use included"
 
 @[rocq_alias frac_agree_includedN]
 theorem includedN {q₁ q₂ : Qp} {a₁ a₂ : A} :
