Iris/Iris/Algebra/ReservationMap.lean
@@ -246,32 +246,33 @@ instance : UCMRA (ReservationMap A H) where
         refine .inr fun HK => bb ?_
         refine (mem_iff_of_validN_union (validN_token_of_validN v) i).mpr ?_
         exact .inl HK
-  assoc := fun n => ⟨CMRA.assoc n, CMRA.assoc n⟩
-  comm := fun n => ⟨CMRA.comm n, CMRA.comm n⟩
-  pcore_op_left {x cx} h := by
+  assoc := Equiv.to_eq <| by refine fun _ => ⟨?_, ?_⟩ <;> exact CMRA.assoc.dist
+  comm := Equiv.to_eq <| by refine fun _ => ⟨?_, ?_⟩ <;> exact CMRA.comm.dist
+  pcore_op_left {x cx} h := Equiv.to_eq <| by
     refine fun n => ⟨?_, ?_⟩
     · simp only [←Option.some_inj.mp h, op_data', core_data]; exact (core_op x.data) n
     · simp [←Option.some_inj.mp h, op_token', core_token, core_op_L]
-  pcore_idem {x cx} h := by
+  pcore_idem {x cx} h := Equiv.to_eq <| by
     refine fun n => ⟨?_, ?_⟩
     · simp only [←Option.some_inj.mp h, core_data]; exact (core_idem x.data) n
     · simp [←Option.some_inj.mp h, core_token, core_idem_L]
   pcore_op_mono {x cx} h y := by
     obtain ⟨z, hz⟩ := core_op_mono x.data y.data
     obtain ⟨w, hw⟩ := core_op_mono x.token y.token
-    refine ⟨mk z w, fun n => ⟨?_, ?_⟩⟩
-    · simp only [op_data', core_data, (Option.some_inj.mp h.symm)]; exact hz n
-    · simp only [core_token, op_token', (Option.some_inj.mp h.symm)]; exact hw n
+    refine ⟨mk z w, Equiv.to_eq ?_⟩
+    refine fun n => ⟨?_, ?_⟩
+    · simp only [op_data', core_data, (Option.some_inj.mp h.symm)]; exact hz.dist
+    · simp only [core_token, op_token', (Option.some_inj.mp h.symm)]; exact hw.dist
   extend {n x y₁ y₂} v exy := by
     obtain ⟨z₁, z₂, xzz, zy₁, zy₂⟩ := CMRA.extend (validN_data_of_validN v) exy.left
-    exact ⟨mk z₁ y₁.token, mk z₂ y₂.token, (fun m => ⟨xzz m, exy.right⟩),
-      ⟨zy₁, rfl⟩, ⟨zy₂, rfl⟩⟩
+    refine ⟨mk z₁ y₁.token, mk z₂ y₂.token, Equiv.to_eq ?_, ⟨zy₁, rfl⟩, ⟨zy₂, rfl⟩⟩
+    exact fun m => ⟨xzz.dist, exy.right⟩
   unit := mk ∅ ∅
   unit_valid := ⟨Heap.valid_empty, fun _ => .inr CoPset.mem_empty⟩
-  unit_left_id {x} := by
+  unit_left_id {x} := Equiv.to_eq <| by
     refine fun n => ⟨?_, (pcore_op_left' (OFE.Equiv.of_eq rfl)) n⟩
     exact (Algebra.MonoidOps.op_left_id : (∅ : H A) • x.data ≡ x.data) n
-  pcore_unit := fun n => ⟨Heap.core_empty n, .rfl⟩
+  pcore_unit := Equiv.to_eq <| by exact fun n => ⟨Heap.core_empty.dist, .rfl⟩
 
 @[simp]
 theorem op_data (x y : ReservationMap A H): (x • y).data = x.data • y.data := rfl
@@ -288,24 +289,29 @@ instance [CMRA.Discrete A] : CMRA.Discrete (ReservationMap A H) where
     · exact validN_disj v
 
 instance instCoreIdSingleton {a : A} [CoreId a] : CoreId (singleton (H := H) k a) where
-  core_id := by
+  core_id := Equiv.to_eq <| by
     refine fun n => OFE.some_dist_some.mpr ⟨?_, .rfl⟩
     exact (core_eqv_self (PartialMap.singleton k a : H A)) n
 
 theorem split_valid {x : ReservationMap A H} (vx : ✓ x) :
-    ∃ (d : H A) (t : CoPset), x ≡ mkData d • mkToken t := by
+    ∃ (d : H A) (t : CoPset), x = mkData d • mkToken t := by
   rcases x with ⟨xd, xt⟩
   match hh : xt with
   | .error =>
     exact ((not_valid_invalid (S := CoPset)) (hh ▸ (valid_token_of_valid vx))).elim
   | .valid t =>
-    refine ⟨xd, t, fun n => ⟨?_, ?_⟩⟩
-    · exact (show xd ≡ xd • (∅ : H A) from Algebra.MonoidOps.op_right_id.symm) n
+    refine ⟨xd, t, ?_⟩
+    apply OFE.Equiv.to_eq
+    refine fun n => ⟨?_, ?_⟩
+    · simp only [mkData, mkToken, op_data]
+      exact (Algebra.MonoidOps.op_right_id.symm) n
     · simp only [mkData, mkToken, op_token]
       exact Dist.of_eq (pcore_op_left_L rfl).symm
 
 theorem split_validN {x : ReservationMap A H} (vx : ✓{n} x) :
-    ∃ (d : H A) (t : CoPset), x ≡ mkData d • mkToken t := by
+    ∃ (d : H A) (t : CoPset), x = mkData d • mkToken t := by
+  suffices h : ∃ (d : H A) (t : CoPset), x ≡ mkData d • mkToken t by
+    obtain ⟨d, t, h⟩ := h; exact ⟨d, t, h.to_eq⟩
   rcases x with ⟨xd, xt⟩
   have H := validN_token_of_validN vx
   match hh : xt with
@@ -333,19 +339,27 @@ theorem validN_singleton (k : Pos) (a : A) : ✓{n} (singleton (H := H) k a) ↔
 theorem valid_token : ✓ (mkToken (H := H) (A := A) e) :=
   ⟨Heap.valid_empty, fun i => .inl (get?_empty i)⟩
 
-theorem data_op (a b : H A) : mkData (a • b) ≡ mkData a • mkData b :=
-  fun _ => ⟨.rfl, Dist.of_eq (pcore_op_right_L rfl).symm⟩
+theorem data_op (a b : H A) : mkData (a • b) = mkData a • mkData b := by
+  apply OFE.Equiv.to_eq
+  refine fun n => ⟨?_, ?_⟩
+  · simp only [mkData, op_data]; exact .rfl
+  · simp only [mkData, op_token]
+    exact Dist.of_eq (pcore_op_left_L rfl).symm
 
 @[rocq_alias reservation_map_data_op]
 theorem singleton_op k (a b : A) :
-    singleton (H := H) k (a • b) ≡ singleton (H := H) k a • singleton k b := by
-  refine ((data_op _ _).symm.trans ?_).symm
-  exact NonExpansive.eqv (fun n i => Dist.of_eq (Heap.singleton_op_singleton i))
+    singleton (H := H) k (a • b) = singleton (H := H) k a • singleton k b := by
+  have he : (({[k := a]} : H A) • {[k := b]}) ≡ {[k := a • b]} :=
+    fun n i => Dist.of_eq (Heap.singleton_op_singleton i)
+  exact (congrArg mkData he.to_eq.symm).trans (data_op _ _)
 
 theorem token_op (a b : CoPset) (h : a ## b) :
-    mkToken (H := H) (A := A) (a ∪ b) ≡ mkToken a • mkToken b := by
-  refine fun n => ⟨(show ∅ ≡ (∅ : H A) • ∅ from Algebra.MonoidOps.op_left_id.symm) n, ?_⟩
-  simp [mkToken, CMRA.op, op_token', h]
+    mkToken (H := H) (A := A) (a ∪ b) = mkToken (H := H) (A := A) a • mkToken b := by
+  apply OFE.Equiv.to_eq
+  refine fun n => ⟨?_, ?_⟩
+  · simp only [mkToken, op_data]
+    exact (Algebra.MonoidOps.op_left_id.symm) n
+  · simp [mkToken, CMRA.op, h]
 
 theorem disj_of_validN_data_op_token {a : H A} {b : CoPset} (h : ✓{n} mkData a • mkToken b) (i : Pos) :
     get? a i = none ∨ i ∉ b := by
@@ -391,24 +405,25 @@ theorem valid_data_op_token (a : H A) (b : CoPset) (vd : ✓ mkData a)
 @[rocq_alias reservation_map_data_mono]
 theorem singleton_mono {k} {a b : A} (Hab : a ≼ b) : singleton (H := H) k a ≼ singleton k b :=
   let ⟨z, hz⟩ := Hab
-  ⟨singleton k z, (NonExpansive.eqv hz).trans (singleton_op k a z)⟩
+  ⟨singleton k z, (congrArg (singleton k) hz).trans (singleton_op k a z)⟩
 
 set_option synthInstance.checkSynthOrder false in
 @[rocq_alias reservation_map_data_is_op]
 instance {ia ib₁ ib₂ : ProofMode.InOut} {a b₁ b₂ : A} [hv : IsOp ia a ib₁ b₁ ib₂ b₂] :
     IsOp ia (singleton (H := H) k a) ib₁ (singleton k b₁) ib₂ (singleton k b₂) where
-  is_op := .trans (NonExpansive.eqv hv.is_op ) (singleton_op k b₁ b₂)
+  is_op := (congrArg (singleton k) hv.is_op).trans (singleton_op k b₁ b₂)
 
 @[rocq_alias reservation_map_token_union]
 theorem token_union {e₁ e₂} (he : e₁ ## e₂) :
-    mkToken (H := H) (A := A) (e₁ ∪ e₂) ≡ mkToken e₁ • mkToken e₂ := by
+    mkToken (H := H) (A := A) (e₁ ∪ e₂) = mkToken (H := H) (A := A) e₁ • mkToken e₂ := by
+  apply OFE.Equiv.to_eq
   refine fun n => ⟨fun i => ?_, ?_⟩
   · simpa only [mkToken, get?_empty, op_data, Heap.get?_op] using .rfl
   · simp [mkToken, CMRA.op, he]
 
 @[rocq_alias reservation_map_token_difference]
 theorem token_difference {e₁ e₂} (he : e₁ ⊆ e₂) :
-    mkToken (H := H) (A := A) e₂ ≡ mkToken e₁ • mkToken (e₂ \ e₁) := by
+    mkToken (H := H) (A := A) e₂ = mkToken (H := H) (A := A) e₁ • mkToken (e₂ \ e₁) := by
   refine .trans ?_ (token_union LawfulSet.disjoint_diff_right)
   rw [LawfulSet.subset_union_diff he]
 
@@ -416,7 +431,7 @@ theorem token_difference {e₁ e₂} (he : e₁ ⊆ e₂) :
 theorem valid_token_op_iff_disj {e₁ e₂} :
     ✓ (mkToken (H := H) (A := A) e₁ • mkToken e₂) ↔ e₁ ## e₂ :=
   ⟨fun h => valid_op_iff_disj.mp (valid_token_of_valid h),
-   fun h => (Equiv.valid (token_union h)).mp valid_token⟩
+   fun h => (Equiv.valid (@OFE.Equiv.of_eq (ReservationMap A H) CMRA.toOFE _ _ (token_union h))).mp valid_token⟩
 
 theorem validN_token_op_iff_disj {e₁ e₂} :
     ✓{n} (mkToken (H := H) (A := A) e₁ • mkToken e₂) ↔ e₁ ## e₂ where
@@ -442,7 +457,7 @@ theorem valid_op?_of_valid_singleton_op {a : A} {x : H A} (h : ✓{n} (singleton
 
 theorem valid_singleton_op_of_valid_op? {a : A} {x : H A} (vx : ✓{n} x) (h : ✓{n} a •? get? x k) :
     ✓{n} singleton k a • mkData x := by
-  refine validN_of_eqv (data_op (PartialMap.singleton k a) x) ?_
+  refine validN_of_eqv (@OFE.Equiv.of_eq (ReservationMap A H) CMRA.toOFE _ _ (data_op (PartialMap.singleton k a) x)) ?_
   refine (validN_data).mpr fun i => ?_
   rw [Heap.get?_op]
   by_cases ki : k = i
@@ -456,22 +471,23 @@ theorem alloc {e k} {a : A} (hke : k ∈ e) (va : ✓ a) : mkToken (H := H) e ~~
   | none => exact Valid.validN <| (valid_singleton k a).mpr va
   | some z =>
     have ⟨d, t, ze⟩ := split_validN (validN_op_right vo)
+    replace ze := @OFE.Equiv.of_eq (ReservationMap A H) CMRA.toOFE _ _ ze
     have vedt : ✓{n} mkToken e • (mkData d • mkToken t) := validN_of_eqv (op_right_eqv _ ze) vo
     have disj : ∀ (i : Pos), get? d i = none ∨ ¬i ∈ e:=
-      disj_of_validN_data_op_token (validN_of_eqv comm (validN_op_left (validN_of_eqv assoc vedt)))
+      disj_of_validN_data_op_token (validN_of_eqv comm' (validN_op_left (validN_of_eqv assoc' vedt)))
     refine validN_of_eqv (op_right_eqv _ ze.symm) ?_
-    refine validN_of_eqv CMRA.assoc.symm ?_
-    refine validN_of_eqv (op_left_eqv (mkToken t) (data_op _ _)) ?_
+    refine validN_of_eqv assoc'.symm ?_
+    refine validN_of_eqv (op_left_eqv (mkToken t) (@OFE.Equiv.of_eq (ReservationMap A H) CMRA.toOFE _ _ (data_op _ _))) ?_
     refine validN_data_op_token (PartialMap.singleton k a • d) t ?_ ?_
-    · refine validN_of_eqv (data_op _ _).symm ?_
+    · refine validN_of_eqv (@OFE.Equiv.of_eq (ReservationMap A H) CMRA.toOFE _ _ (data_op _ _).symm) ?_
       apply valid_singleton_op_of_valid_op?
-      · exact validN_data.mp (validN_op_left (validN_of_eqv comm (validN_op_left (validN_of_eqv assoc vedt))))
+      · exact validN_data.mp (validN_op_left (validN_of_eqv comm' (validN_op_left (validN_of_eqv assoc' vedt))))
       · exact (disj k).elim (fun h => h ▸ Valid.validN va) (absurd hke)
     · simp only [CMRA.op, Heap.op, get?_merge, LawfulPartialMap.get?_singleton,
         Option.merge_eq_none_iff, ite_eq_right_iff, reduceCtorEq, imp_false]
       intro i
       grind [disj_of_validN_data_op_token (validN_of_eqv ze (validN_op_right vo)),
-        validN_token_op_iff_disj.mp (validN_op_right (validN_of_eqv assoc.symm (validN_of_eqv comm vedt))) i]
+        validN_token_op_iff_disj.mp (validN_op_right (validN_of_eqv assoc'.symm (validN_of_eqv comm' vedt))) i]
 
 @[rocq_alias reservation_map_updateP]
 theorem updateP {P} {Q : ReservationMap A H → Prop} k a (ap : a ~~>: P)
@@ -483,24 +499,25 @@ theorem updateP {P} {Q : ReservationMap A H → Prop} k a (ap : a ~~>: P)
     exact ⟨_, (apq y py), (validN_singleton k y).mpr vy⟩
   | some z =>
     obtain ⟨d, t, ze⟩ := split_validN (validN_op_right vaz)
+    replace ze := @OFE.Equiv.of_eq (ReservationMap A H) CMRA.toOFE _ _ ze
     obtain ⟨y, py, vy⟩ := ap n (get? d k)
       (valid_op?_of_valid_singleton_op
-        (validN_op_left (validN_of_eqv CMRA.assoc
+        (validN_op_left (validN_of_eqv assoc'
           (validN_of_eqv (op_right_eqv (singleton k a) ze) vaz))))
     refine ⟨singleton k y, apq y py, ?_⟩
     simp only [CMRA.op?] at vaz ⊢
     refine validN_of_eqv (op_right_eqv (singleton k y) ze).symm ?_
-    refine validN_of_eqv CMRA.assoc.symm ?_
-    refine validN_of_eqv (op_left_eqv (mkToken t) (data_op _ _)) ?_
+    refine validN_of_eqv assoc'.symm ?_
+    refine validN_of_eqv (op_left_eqv (mkToken t) (@OFE.Equiv.of_eq (ReservationMap A H) CMRA.toOFE _ _ (data_op _ _))) ?_
     refine validN_data_op_token _ _ ?_ ?_
-    · refine validN_of_eqv (data_op _ _).symm ?_
+    · refine validN_of_eqv (@OFE.Equiv.of_eq (ReservationMap A H) CMRA.toOFE _ _ (data_op _ _).symm) ?_
       refine valid_singleton_op_of_valid_op? ?_ vy
       refine validN_data.mp ?_
       exact validN_op_left $ validN_of_eqv ze (validN_op_right vaz)
     · have ddt := disj_of_validN_data_op_token (validN_of_eqv ze (validN_op_right vaz))
-      have dde := disj_of_validN_data_op_token <| validN_of_eqv CMRA.comm
-        (validN_op_right (validN_of_eqv CMRA.assoc.symm
-          (validN_of_eqv CMRA.comm (validN_of_eqv (CMRA.cmra_op_ne2.eqv .rfl ze) vaz))))
+      have dde := disj_of_validN_data_op_token <| validN_of_eqv comm'
+        (validN_op_right (validN_of_eqv assoc'.symm
+          (validN_of_eqv comm' (validN_of_eqv (CMRA.cmra_op_ne2.eqv .rfl ze) vaz))))
       simp only [CMRA.op, Heap.op, get?_merge, LawfulPartialMap.get?_singleton,
         Option.merge_eq_none_iff, ite_eq_right_iff, reduceCtorEq, imp_false] at ddt dde ⊢
       grind
